Finish expression transformation function; start proofs of equivalence.

proof-of-soundness/c-subset-syntax.v
@@ -14,22 +14,13 @@ Definition state : Set := @list (nat * Z).
    the corresponding L-value wrapped in an option type if found;
    otherwise returns None *)
 Definition lookupE (x:string) (E:environment) : option nat :=
-  match find (fun pair => String.eqb (fst pair) x) E with
-  | None => None
-  | Some (_, l) => Some l
-  end.
+  option_map snd (find (fun pair => String.eqb (fst pair) x) E).
 
 (* Looks up an L-value in the store and returns
    the corresponding R-value wrapped in an option type if found;
    otherwise returns None *)
 Definition lookupS (l:nat) (S:state) : option Z :=
-  match find (fun pair => Nat.eqb (fst pair) l) S with
-  | None => None
-  | Some (_, z) => Some z
-  end.
-
-(* Compute (find (fun s => s =? "s") (nil)). *)
-(* Compute (find (fun s => s =? "s") (cons "s" (nil))). *)
+  option_map snd (find (fun pair => Nat.eqb (fst pair) l) S).
 
 (* Unary operators *)
 Inductive unop : Type :=
@@ -74,8 +65,7 @@ Inductive expr : Type :=
   | UnExpr (uo : unop) (e : expr)
   | BinExpr (bo : binop) (e1 e2 : expr)
   | Assign (x: string) (e : expr)
-  | FunctionCall (x : string) (es: list expr)
-  | MacroInvocation (x : string) (es: list expr).
+  | CallOrInvocation (x : string) (es: list expr).
 
 Inductive stmt : Type :=
   (* We may not need this, I added it to make the evaluation rule
@@ -94,57 +84,60 @@ Inductive decl : Type :=
   | GlobalDecl (x:string) (ce:const_expr).
 
 (* Mappings from function and macro names to their definitions *)
-(* Functions are defined as a 4-tuple:
-   0: List of parameter names
-   1: List of declarations
-   2: List of statements
-   3: Return expressions
-*)
-(* This is actually kind of ugly, because it says that a function
-   definition could be a list of declarations, which could each
-   either be global or local. Since they are inside a function body,
-   however, of course they are local. How to rectify this? *)
+(* Functions are defined as a 3-tuple:
+   0: Environment which contains processed local declarations and
+      parameters
+   1: Body that is a statement (could be a compound statement)
+   2: Return expression *)
+(* TODO: Eventually we may want to swap the environment out for a
+         parameter list and operate on that instead *)
 Definition func_definition : Set :=
-  ((list string) * (list decl) * (list stmt) * expr).
+  (environment * stmt * expr).
 Definition func_definitions : Set := @list (string * func_definition).
 
-(* Macro definitions are serialized as a two-tuple containing a
-   list of their parameter names and their macro body
-   (a single expression) *)
-Definition macro_body : Set := ((list string) * expr).
-Definition macro_bodies : Set := @list (string * macro_body).
+(* Macro definitions are serialized as a two-tuple containing
+   the macros parameters mapped to their arguments (the environment)
+   and the macro body (a single expression).
+   TODO: This does not exactly model how macros work. To fix this,
+         we will need to swap out the environment for a list of
+         parameters and the body for something more akin to what we
+         have for functions.
+   *)
+Definition macro_definition : Set := (environment * expr).
+Definition macro_definitions : Set := @list (string * macro_definition).
 
 (* Looks up a function name in the function defintion list and returns
    the corresponding definition wrapped in an option type if found;
    otherwise returns None *)
 Definition definition
   (x:string) (defs:func_definitions) : option func_definition :=
-  match find (fun pair => String.eqb (fst pair) x) defs with
-  | None => None
-  | Some (_, def) => Some def
-  end.
+  option_map snd (find (fun pair => String.eqb (fst pair) x) defs).
 
 (* Looks up a macro name in the function defintion list and returns
    the corresponding definition wrapped in an option type if found;
    otherwise returns None *)
 Definition invocation
-  (x:string) (defs:macro_bodies) : option macro_body :=
-  match find (fun pair => String.eqb (fst pair) x) defs with
-  | None => None
-  | Some (_, body) => Some body
-  end.
+  (x:string) (defs:macro_definitions) : option macro_definition :=
+  option_map snd (find (fun pair => String.eqb (fst pair) x) defs).
 
 (* Right now, a term that fails to evaluate will simply get "stuck";
-   we do not provide any error messages. I think we could add this
+   i.e. it will fail to be reduced further.
+   We do not provide any error messages, but I think we could add this
    later using a sum type. *)
+(* TODO: Add G, the global environment *)
+
+Open Scope Z_scope.
+
 Reserved Notation
   "[ S , E , F , M '|-' e '=>' v , S' ]"
   (at level 90, left associativity).
-
-Inductive eevalR :
-  state -> environment -> func_definitions -> macro_bodies ->
-  expr -> Z ->
-  state -> Prop :=
+Reserved Notation
+  "{ S , E , F , M '=[' s ']=>' S' }"
+  (at level 91, left associativity).
+Inductive exprevalR :
+  state -> environment -> func_definitions -> macro_definitions ->
+  expr ->
+  Z -> state -> Prop :=
   (* Variable lookup returns the variable's R-value
      and does not change the state *)
   | E_X_Success : forall S E F M x l v,
@@ -185,55 +178,270 @@ Inductive eevalR :
   (* For function calls, each of the function call's arguments are
      evaluated, then the function call itself is evaluated, and finally
      the result of the call is returned along with the ultimate state. *)
-  (* TODO *)
-  | E_FunctionCall: forall S E F M x es def,
-    definition x F = Some def ->
-    [S, E, F, M |- (FunctionCall x es) => 0, S]
-  (* Macro invocation, no side-effects *)
-  (* TODO *)
-  | E_MacroInvocationNoSideEffects : forall S E F M x es body,
-    invocation x M = Some body ->
-    [S, E, F, M |- (MacroInvocation x es) => 0, S]
-  where "[ S , E , F , M '|-' e '=>' v , S' ]" := (eevalR S E F M e v S') : type_scope.
-
-(* TODO: Fix evaluation rules for statements *)
-
-Open Scope Z_scope.
-
-Reserved Notation
-  "[ S , E , F , M '=[' s ']=>' S' ]"
-  (at level 91, left associativity).
+  | E_FunctionCall: forall S E F M x es fenv fstmt fexpr S' v S'',
+    definition x F = Some (fenv, fstmt, fexpr) ->
+    {S, fenv, F, M =[ fstmt ]=> S'} ->
+    [S, fenv, F, M |- fexpr => v, S''] ->
+    [S, E, F, M |- (CallOrInvocation x es) => v, S'']
+  (* Macro invocation*)
+  (* FIXME *)
+  | E_MacroInvocation : forall S E F M x es menv mexpr v S',
+    invocation x M = Some (menv, mexpr) ->
+    [S, menv, F, M |- mexpr => v, S'] ->
+    [S, E, F, M |- (CallOrInvocation x es) => v, S']
+  where "[ S , E , F , M '|-' e '=>' v , S' ]" := (exprevalR S E F M e v S')
 (* Define the evaluation rule for statements as a
    relation instead of an inductive type to permite the non-
    determinism introduced by while loops *)
-Inductive stmtevalR :
-  state -> environment -> func_definitions -> macro_bodies ->
+with stmtevalR :
+  state -> environment -> func_definitions -> macro_definitions ->
   stmt ->
   state -> Prop :=
   (* A skip statement does not change the state *)
   | E_Skip : forall S E F M,
-    [S, E, F, M =[ Skip ]=> S]
+    {S, E, F, M =[ Skip ]=> S}
   (* An expression statement evaluates its expression and returns 
      the resulting state *)
   | E_ExprStmt : forall S E F M e v S',
-    eevalR S E F M e v S' ->
-    [S, E, F, M =[ ExprStmt e ]=> S']
+    exprevalR S E F M e v S' ->
+    {S, E, F, M =[ ExprStmt e ]=> S'}
   (* An empty compound statement evaluates to its initial state *)
   | E_CompoundStatementEmpty : forall S E F M,
-    [S, E, F, M =[ CompoundStmt nil ]=> S]
-  | E_CompoundStatementNotEmpty : forall S  E F M stmts s0 rst S' S'',
+    {S, E, F, M =[ CompoundStmt nil ]=> S}
+  (* A non-empty compound statement evaluates its first statement and
+     then the following statements *)
+  | E_CompoundStatementNotEmpty : forall S E F M stmts s0 rst S' S'',
     head stmts = Some s0 ->
     tail stmts = rst ->
-    [S, E, F, M =[ s0 ]=> S'] ->
-    [S', E, F, M =[ CompoundStmt rst ]=> S''] ->
-    [S', E, F, M =[ CompoundStmt stmts ]=> S'']
-  (* TODO: If statement *)
-  (* TODO: If else statement *)
-  (* TODO: While statement *)
-  
-  where "[ S , E , F , M '=[' s ']=>' S' ]" := (stmtevalR S E F M s S') : type_scope.
+    {S, E, F, M =[ s0 ]=> S'} ->
+    {S', E, F, M =[ CompoundStmt rst ]=> S''} ->
+    {S, E, F, M =[ CompoundStmt stmts ]=> S''}
+  (* An if statement whose condition evaluates to false only carries
+     over the side-effects induced by evaluating its condition *)
+  | E_IfFalse: forall S E F M e s0 S',
+    [S, E, F, M |- e => 0, S'] ->
+    {S, E, F, M =[ IfStmt e s0 ]=> S'}
+  (* An if statement whose condition evaluates to true carries over
+     the side-effects from evaluating its condition and its statement *)
+  | E_IfTrue: forall S E F M e s0 v S' S'',
+    v <> 0 ->
+    [S, E, F, M |- e => v, S'] ->
+    {S',E, F, M =[ s0 ]=> S''} ->
+    {S, E, F, M =[ IfStmt e s0 ]=> S''}
+  (* Side-effects from condition and false branch *)
+  | E_IfElseFalse: forall S E F M e s0 s1 S' S'',
+    [S, E, F, M |- e => 0, S'] ->
+    {S',E, F, M =[ s1 ]=> S''} ->
+    {S, E, F, M =[ IfElseStmt e s0 s1 ]=> S''}
+  (* Side-effects from condition and true branch *)
+  | E_IfElseTrue: forall S E F M e s0 s1 v S' S'',
+    v <> 0 ->
+    [S, E, F, M |- e => v, S'] ->
+    {S',E, F, M =[ s0 ]=> S''} ->
+    {S, E, F, M =[ IfElseStmt e s0 s1 ]=> S''}
+  (* Similar to E_IfFalse *)
+  | E_WhileFalse: forall S E F M e s0 S',
+    [S, E, F, M |- e => 0, S'] ->
+    {S, E, F, M =[ WhileStmt e s0 ]=> S'}
+  (* A while statement whose condition evaluates to false must be run
+     again after evaluating its body *)
+  | E_WhileTrue: forall S E F M e s0 v S' S'' S''',
+    v <> 0 ->
+    [S, E, F, M |- e => v, S'] ->
+    {S', E, F, M =[ s0 ]=> S''} ->
+    {S'', E, F, M =[ WhileStmt e s0 ]=> S'''} ->
+    {S, E, F, M =[ WhileStmt e s0 ]=> S'''}
+  where "{ S , E , F , M '=[' s ']=>' S' }" := (stmtevalR S E F M s S').
 
 Close Scope Z_scope.
+
+(* Returns true if an expression has side-effects, false otherwise *)
+Definition has_side_effects (e : expr) : bool. Admitted.
+
+(* Returns the list of dynamic variables used within
+   a macro definition *)
+(* TODO: Fix this to actually work. It will probably need the caller
+   environment added to its parameter list.
+   This will in turn necessitate adding the caller environment to
+   transform function below, since that is where this function is
+   used *)
+Definition get_dynamic_vars (md : macro_definition) : list string.
+Admitted.
+
+Fixpoint transform
+  (F: func_definitions) (M: macro_definitions) (e:expr) : 
+  (func_definitions * macro_definitions * expr) :=
+  match e with
+ (* Don't transform variables *)
+ | X x => (F, M, X x)
+ (* Don't transform numerals *)
+ | Num z => (F, M, Num z)
+ (* Transform the inner expression of a parenthesize expression *)
+ | ParenExpr e =>
+    let '(F', M', e') := (transform F M e) in
+      (F', M', ParenExpr e')
+ (* Transform the operand of a unary expressions *)
+ | UnExpr uo e => 
+    let '(F', M', e') := (transform F M e) in
+      (F', M', UnExpr uo e')
+ (* Transform the operands of a binary expressions *)
+ | BinExpr bo e1 e2 =>
+    let '(F', M', e1') := transform F M e1 in
+      let '(F'', M'', e2') := (transform F' M' e2) in
+         (F'', M'', BinExpr bo e1' e2')
+ (* Transform the expression of an assignment *)
+ (* (this will have to change if L-value evaluation is added *)
+ | Assign x e =>
+    let '(F', M', e') := (transform F M e) in
+      (F', M', Assign x e')
+ (* Transformation here varies whether a function or macro invocation
+    is being called *)
+ | CallOrInvocation x es =>
+    match definition x F with
+    (* If this identifier maps to a function definition, then the
+       original piece of code was a function call.
+       We don't transform functions, but since each of the function
+       call arguments are expressions, we have to iterate over and
+       transform each of them.
+       We implement this iteration via a right fold to avoid
+       having to reverse the list afterward. *)
+    | Some def =>
+      let '(finalF, finalM, finalList) :=
+      fold_right (
+        fun e acc =>
+          let '(lastF, lastM, lastList) := acc in
+            let '(newF, newM, newe) := (transform lastF lastM e) in
+              (newF, newM, newe::lastList)
+        ) (F, M, nil) es in
+          (finalF, finalM, CallOrInvocation x finalList)
+    | None =>
+        match invocation x M with
+        | Some (menv, mexpr) =>
+          (* add guard clauses for different transformations *)
+          (* need a way of generating a fresh name *)
+          (* Do any of the the macro arguments have side_effects? *)
+          match existsb has_side_effects es with
+            (* If not, then proceed with other checks *)
+            | false =>
+              (* Does the macro body have side-effects? *)
+              match has_side_effects mexpr with
+              | false =>
+                (* Does the macro use dynamic scoping? *)
+                match get_dynamic_vars (menv, mexpr) with
+                (* No, so just transform the macro to a function *)
+                | nil =>
+                  (* Don't remove from M; copy a new definition
+                     to just F *)
+                  let fname := x ++ "__as_function" in
+                    let F' := (fname, (menv, Skip, mexpr))::F in
+                      (F', M, CallOrInvocation fname es)
+                (* Yes, so add the dynamic variables to the transformed
+                   function's parameter list *)
+                | dyn_vars => (F, M, e) (* FIXME *)
+                end
+              | true =>
+                (* Does the macro use dynamic scoping? *)
+                match get_dynamic_vars (menv, mexpr) with
+                (* No, so just transform the macro to a function *)
+                | nil => (F, M, e) (* FIXME *)
+                (* Yes, so add the dynamic variables to the transformed
+                   function's parameter list *)
+                | dyn_vars => (F, M, e) (* FIXME *)
+                end
+              end
+            (* If so, then don't transform the macro *)
+            | true => (F, M, e)
+            end
+        (* If a call can't be connected to a function or macro, then
+           it's erroneous anyway so leave it as-is *)
+        | None => (F, M, e)
+        end
+      end
+ end.
+
+
+(* Variables are equivalent under transformation *)
+Fact var_eq_transformed :
+  forall (S S': state) (E : environment)
+         (F F': func_definitions) (M M': macro_definitions)
+         (e e': expr) (x : string) (v : Z),
+  e = X x ->
+  transform F M e = (F', M', e') ->
+  exprevalR S E F M e v S' = exprevalR S E F' M' e' v S'.
+Proof.
+  intros.
+  rewrite H in H0. simpl in H0. rewrite <- H in H0.
+  inversion H0.
+  reflexivity.
+Qed.
+
+(* Numerals are equivalent under transformation *)
+Theorem num_eq_transformed : 
+  forall (S S': state) (E : environment)
+         (F F': func_definitions) (M M': macro_definitions)
+         (e e': expr) (v z: Z),
+  e = Num z ->
+  transform F M e = (F', M', e') ->
+  exprevalR S E F M e v S' = exprevalR S E F' M' e' v S'.
+Proof.
+  intros.
+  rewrite H in H0. simpl in H0. rewrite <- H in H0.
+  inversion H0.
+  reflexivity.
+Qed.
+
+(* A parenthesized expression whose inner expression is equivalent
+   under transformation is also equivalent under transformation *)
+Theorem paren_expr_eq_transformed : 
+  forall (S S' S'': state) (E : environment)
+         (F F0' F': func_definitions) (M M0' M': macro_definitions)
+         (e innerExpr innerExpr' e': expr) (v: Z),
+  e = ParenExpr innerExpr ->
+  transform F M innerExpr = (F0', M0', innerExpr') ->
+  (F, M, innerExpr) = (F0', M0', innerExpr') ->
+  exprevalR S E F M innerExpr v S' = exprevalR S E F0' M0' innerExpr' v S' ->
+  transform F0' M0' e = (F', M', e') ->
+  exprevalR S' E F M e v S'' = exprevalR S' E F' M' e' v S''.
+Proof.
+  intros.
+  inversion H1.
+  rewrite H in H3. simpl in H3.
+  rewrite <- H5 in H3. rewrite <- H6 in H3. rewrite H0 in H3.
+  inversion H3. rewrite <- H7. rewrite <- H. reflexivity.
+Qed.
+
+(* A call to a macro without side-effects is equivalent to a call
+   to the transformed version of that macro as a function *)
+Theorem func_call_eq_transformed_macro_no_side_effects : 
+  forall (S S': state) (E menv : environment)
+         (F F': func_definitions) (M M': macro_definitions)
+         (e mexpr e': expr) (x fname : string) (es : list expr)
+         (v : Z),
+  e = CallOrInvocation x es ->
+  definition x F = None ->
+  invocation x M = Some (menv, mexpr) ->
+  existsb has_side_effects es = false ->
+  has_side_effects mexpr = false ->
+  get_dynamic_vars (menv, mexpr) = nil ->
+  fname = x ++ "__as_function" ->
+  transform F M e = (F', M', e') ->
+  definition fname F = Some (menv, Skip, mexpr) ->
+  (* This premise is VERY strong, can we weaken it?
+     Here we assume that a call to the macro will result
+     in the same value and state as a call to the
+     transformed function will. *)
+  exprevalR S E F M (CallOrInvocation x es) v S' =
+  exprevalR S E F' M' (CallOrInvocation fname es) v S' ->
+  exprevalR S E F M e v S' = exprevalR S E F' M' e' v S'.
+Proof.
+  intros.
+  rewrite H in H6. simpl in H6.
+  rewrite H0, H1, H2, H3, H4 in H6.
+  rewrite <- H5 in H6.
+  inversion H6.
+  simpl. rewrite H. pattern M' at 1; rewrite <- H11. rewrite H10.
+  rewrite H8. reflexivity.
+Qed.
 
 
 Close Scope string_scope.
